**Class**: [[COMP1600 - Theoretical Computer Science]]
**Date**: Wednesday, 6 August 2025, 10:03
**Tags**: 

---
#### Lecture 1
ToDo

#### Lecture 2
##### Proof Strategies
- Proving $A \implies B$ 
	- Assume $A$ is true.
	- Prove $B$ using that assumption.
```c
if (A){
  // proof of B using A.
  assert (A ==> B);
  assert(A);
  assert(B);
}
```

##### Proof using Case Split
- All predicates either hold or don't hold. Therefore, we can use this fact.
- Assume $A \lor \neg A$.
- Do a case split where you assume each of the cases.
```c
assert (A || !A)
if (A){
  // proof for A
}
if (!A){
  // proof using !A.
}
```

##### Proof using Existential
- Proving $\exists x. A(x)$ from a set of assumptions
- If $e$ is an expression of the same type as $x$ and $A[e/x](x)$ is true, then $\exists x. A(X)$ holds.
```c
assert P(e) // assuming we have already proved P(e)
assert (exists x:T :: P(x));
```

 You want to declare a new variable, and make it so that it matches the conditions of the function.
 ```c
 var x:T :| P(x);
 // :| = such that
 ```
- Now $x$ and $P(x)$ can be used in the proof. 
 
##### Proof using Universal
- Proving $\forall x.A(x)$ from a set of assumptions.
```c
forall x:T ensures P(x){
  // Proof of P(x)
}
```
- This is like saying: Let there be some $x$ of type $T$, $x:T$, and show $P(x)$
- We need to get a $\forall$ that will give us this property  $P(x)$

- If $e$ is an expression of the same type as $x$, conclude $A(e)$
```c
assert (forall x:T :: P(x)); // asumme this is proved.
assert P(e)
```


##### Examples
- Prove that $\forall m,n \in Z.\text{even}(m)\land\text{even}(n) \implies \text{even}(m+n)$
- Prove for any two integers, the sum of them must be even.

- Suppose that $m$ and $n$ are arbitrary integers that are even.
- Required to show: That $m$ + $n$ is even.
	- How do we show that a number is even?
	- An integer $n$ is even if $n = 2k$ for some integer $k$.
	- $\text{even}(n) \equiv \exists k \in Z.n=2*k$    

- Suppose that $m$ and $n$ are arbitrary integers that are even.
- Therefore, $m = 2 \times i$ and $n = 2 \times j$, for some integers $i$ and $j$.
$$m + n = 2 \times i + 2 \times j = 2(i+j)$$
- Since $i + j$ is an integer, we can set $i + j = v$
- Therefore, $m + n = 2 \times v$
- Therefore, even($m+n$)

##### Examples
- A natural number $n$ divides $m$ if $m = n \times k$, for some natural number $k$.
$$ div(n,m) \equiv \exists k \in N. m=n \times k$$
- Prove that for all integers $x$, $y$, and $z$, if $x$ divides $y$ and $y$ divides $z$, then $x$ divides $z$.
- Required to prove:
$$
\forall x,y,z \in \mathbb{Z}.\; \text{div}(x,y) \land \text{div}(y,z) \;\Rightarrow\; \text{div}(x,z)
$$
- Let $x$, $y$, and $z$ be arbitrary integers, such that $x$ divides $y$ and $y$ divides $z$.
- Therefore, $y = x \times k$ and $z = y \times j$, for some integers $k$ and $j$.
$$
y = x \times k \quad (1)
$$
$$
z = y \times j \quad (2)
$$
- Prove that any two consecutive integers have opposite parity.
- Use the following theorem: **Any integer is either even or odd**.
Required to prove:  
$$
\forall m \in \mathbb{Z}. \; (even(m) \land odd(m+1)) \;\lor\; (even(m+1) \land odd(m))
$$
- Let $m$ and $m+1$ be two arbitrarily chosen consecutive integers.  
- By the above theorem, $m$ is either even or odd.  
- Split it into cases:  
	- Case 1: $even(m)$  
	- Case 2: $odd(m)$  
where  $odd(n) \equiv \exists k \in \mathbb{Z}. \; n = 2 \cdot k + 1$

**Case 1**: $even(m)$  
Therefore, $m = 2 \cdot k$, for some integer $k$.  
$$
m + 1 = (2 \cdot k) + 1, \quad \text{by substitution of } m = 2 \cdot k.
$$
Therefore, $odd(m+1)$, by the definition of $odd$.  

**Case 2**: $odd(m)$  
Therefore, $m = 2 \cdot k + 1$, for some integer $k$.  
$$
\begin{aligned}
m + 1 &= (2 \cdot k + 1) + 1 \\
m + 1 &= 2 \cdot k + 2 \\
m + 1 &= 2 \cdot (k + 1)
\end{aligned}
$$
```c
ghost predicate DividesByFive(x:int) {exists k: int :: x == 5 * k}


lemma addDividesFive()

  ensures forall x:int, y:int, z:int :: DividesByFive(x) && DividesByFive(y) ==> DividesByFive(x * y){

    // If X is divisible by 5, and Y is divisible by 5, then X * Y is divisible by 5.

    forall x:int, y:int, z:int ensures DividesByFive(x) && DividesByFive(y) ==> DividesByFive(x * y){

      if(DividesByFive(x)){

        var k:int  :| x == 5 * k;

        if(DividesByFive(y)){

          var z:int  :| y == 5 * z;

          assert (x * y == (5 * k) * (5 * z));

          assert (x * y == 5 * 5 * k * z);

          assert (x * y == 5 * (5 * k * z));
        }
      }
    }
}
```


#### Lecture 3